Adapt theories importing LNLC_Typing to the refactored type ty
Register a size function for ty_comb before the datatype ty is declared, so
the size plugin descends into a type constructor's arguments; this revives
size_ty_TyCtr/size_ty_TyFun and leaves Red_ty's termination proof unchanged.
Elsewhere, use the const_ty accessors instead of Rep_const_ty, swap the
ty/const_ty parameter order, and rename type_vars to free_vars_ty.
denotation_ty is now a primrec over the ty datatype.

Co-Authored-By: Claude Opus 5 <noreply@anthropic.com>

Locally_Nameless_Lambda_Calculus/LNLC_Semantics.thy
@@ -68,50 +68,32 @@ locale type_valuation = universe +
   fixes \<xi>\<^sub>t\<^sub>y :: "'\<V>\<^sub>t\<^sub>y \<Rightarrow> V"
   assumes \<xi>\<^sub>t\<^sub>y_codom[intro]: "\<And>x. \<xi>\<^sub>t\<^sub>y x \<in> \<U>"
 
-primrec denotation_prety ::
-  "('\<V>\<^sub>t\<^sub>y \<Rightarrow> V) \<Rightarrow> '\<Sigma>\<^sub>t\<^sub>y type_interp_fun \<Rightarrow> ('\<V>\<^sub>t\<^sub>y, '\<Sigma>\<^sub>t\<^sub>y) prety \<Rightarrow> V" where
-  "denotation_prety \<xi>\<^sub>t\<^sub>y \<J>\<^sub>t\<^sub>y (PretyVar \<alpha>) = \<xi>\<^sub>t\<^sub>y \<alpha>" |
-  "denotation_prety \<xi>\<^sub>t\<^sub>y \<J>\<^sub>t\<^sub>y (PretyCtr \<kappa> \<tau>s) = \<J>\<^sub>t\<^sub>y \<kappa> (map (denotation_prety \<xi>\<^sub>t\<^sub>y \<J>\<^sub>t\<^sub>y) \<tau>s)"
+primrec denotation_ty ::
+  "('\<V>\<^sub>t\<^sub>y \<Rightarrow> V) \<Rightarrow> '\<Sigma>\<^sub>t\<^sub>y type_interp_fun \<Rightarrow> ('\<Sigma>\<^sub>t\<^sub>y :: arity, '\<V>\<^sub>t\<^sub>y) ty \<Rightarrow> V" where
+  "denotation_ty \<xi>\<^sub>t\<^sub>y \<J>\<^sub>t\<^sub>y (TyVar \<alpha>) = \<xi>\<^sub>t\<^sub>y \<alpha>" |
+  "denotation_ty \<xi>\<^sub>t\<^sub>y \<J>\<^sub>t\<^sub>y (TyCtr \<kappa>_\<tau>s) =
+    \<J>\<^sub>t\<^sub>y (tycon \<kappa>_\<tau>s) (tyargs (map_ty_comb (denotation_ty \<xi>\<^sub>t\<^sub>y \<J>\<^sub>t\<^sub>y) \<kappa>_\<tau>s))"
 
-definition denotation_ty ::
-  "('\<V>\<^sub>t\<^sub>y \<Rightarrow> V) \<Rightarrow> '\<Sigma>\<^sub>t\<^sub>y type_interp_fun \<Rightarrow> ('\<V>\<^sub>t\<^sub>y, '\<Sigma>\<^sub>t\<^sub>y :: arity) ty \<Rightarrow> V" where
-  "denotation_ty \<xi>\<^sub>t\<^sub>y \<J>\<^sub>t\<^sub>y \<tau> = denotation_prety \<xi>\<^sub>t\<^sub>y \<J>\<^sub>t\<^sub>y (Rep_ty \<tau>)"
+text \<open>The arity invariant of a type constructor application is internal to \<^type>\<open>ty_comb\<close>, so the
+  denotation of a type lands in the universe unconditionally.\<close>
 
-lemma
+lemma denotation_ty_in_universe:
   assumes "type_interp \<U> \<J>\<^sub>t\<^sub>y" and "type_valuation \<U> \<xi>\<^sub>t\<^sub>y"
-  shows
-    denotation_prety_in_universe: "\<And>\<tau>. wf_prety \<tau> \<Longrightarrow> denotation_prety \<xi>\<^sub>t\<^sub>y \<J>\<^sub>t\<^sub>y \<tau> \<in> \<U>" and
-    denotation_ty_in_universe: "\<And>\<tau>. denotation_ty \<xi>\<^sub>t\<^sub>y \<J>\<^sub>t\<^sub>y \<tau> \<in> \<U>"
-proof -
-  show 1: "denotation_prety \<xi>\<^sub>t\<^sub>y \<J>\<^sub>t\<^sub>y \<tau> \<in> \<U>" if "wf_prety \<tau>" for \<tau>
-    using that
-  proof (induction \<tau>)
-    case (PretyVar \<alpha>)
-    then show ?case
-      by (metis assms(2) denotation_prety.simps(1) type_valuation.\<xi>\<^sub>t\<^sub>y_codom)
-  next
-    case (PretyCtr \<kappa> \<tau>s)
-    show ?case
-      unfolding denotation_prety.simps
-    proof (rule type_interp.\<J>\<^sub>t\<^sub>y_codom[OF assms(1)])
-      show "length (map (denotation_prety \<xi>\<^sub>t\<^sub>y \<J>\<^sub>t\<^sub>y) \<tau>s) = arity \<kappa>"
-        using PretyCtr.hyps by simp
-    next
-      show "\<And>\<D>. \<D> \<in> list.set (map (denotation_prety \<xi>\<^sub>t\<^sub>y \<J>\<^sub>t\<^sub>y) \<tau>s) \<Longrightarrow> \<D> \<in> \<U>"
-        using PretyCtr.IH by auto
-    qed
-  qed
-
-  show "denotation_ty \<xi>\<^sub>t\<^sub>y \<J>\<^sub>t\<^sub>y \<tau> \<in> \<U>" for \<tau>
-  proof (cases \<tau>)
-    case (Abs_ty \<tau>')
-    then have "wf_prety \<tau>'"
+  shows "denotation_ty \<xi>\<^sub>t\<^sub>y \<J>\<^sub>t\<^sub>y \<tau> \<in> \<U>"
+proof (induction \<tau>)
+  case (TyVar \<alpha>)
+  show ?case
+    using type_valuation.\<xi>\<^sub>t\<^sub>y_codom[OF assms(2)] by simp
+next
+  case (TyCtr \<kappa>_\<tau>s)
+  show ?case
+    unfolding denotation_ty.simps
+  proof (rule type_interp.\<J>\<^sub>t\<^sub>y_codom[OF assms(1)])
+    show "length (tyargs (map_ty_comb (denotation_ty \<xi>\<^sub>t\<^sub>y \<J>\<^sub>t\<^sub>y) \<kappa>_\<tau>s)) = arity (tycon \<kappa>_\<tau>s)"
       by simp
-    then have "denotation_prety \<xi>\<^sub>t\<^sub>y \<J>\<^sub>t\<^sub>y \<tau>' \<in> \<U>"
-      using 1 by iprover
-    then show ?thesis
-      using Abs_ty
-      by (metis Abs_ty_inverse[of \<tau>'] denotation_ty_def)
+  next
+    show "\<And>\<D>. \<D> \<in> list.set (tyargs (map_ty_comb (denotation_ty \<xi>\<^sub>t\<^sub>y \<J>\<^sub>t\<^sub>y) \<kappa>_\<tau>s)) \<Longrightarrow> \<D> \<in> \<U>"
+      using TyCtr.IH by auto
   qed
 qed
 
@@ -126,14 +108,14 @@ type_synonym '\<Sigma> term_interp_fun = "'\<Sigma> \<Rightarrow> V list \<Right
 
 locale interp_fun = type_interp \<U> \<J>\<^sub>t\<^sub>y
   for \<U> and \<J>\<^sub>t\<^sub>y :: "('\<Sigma>\<^sub>t\<^sub>y :: type_signature) type_interp_fun" +
-  fixes \<C> :: "'\<Sigma> :: term_signature \<Rightarrow> ('\<V>\<^sub>t\<^sub>y, '\<Sigma>\<^sub>t\<^sub>y) const_ty"
+  fixes \<C> :: "'\<Sigma> :: term_signature \<Rightarrow> ('\<Sigma>\<^sub>t\<^sub>y, '\<V>\<^sub>t\<^sub>y) const_ty"
   fixes \<J> :: "'\<Sigma> term_interp_fun"
-  assumes "\<And>(\<xi>\<^sub>t\<^sub>y :: '\<V>\<^sub>t\<^sub>y \<Rightarrow> V) f \<alpha>s \<tau>s v \<D>s as.
+  assumes "\<And>(\<xi>\<^sub>t\<^sub>y :: '\<V>\<^sub>t\<^sub>y \<Rightarrow> V) f \<D>s as.
     type_valuation \<U> \<xi>\<^sub>t\<^sub>y \<Longrightarrow>
-    Rep_const_ty (\<C> f) = (\<alpha>s, \<tau>s, v) \<Longrightarrow> length \<D>s = length \<alpha>s \<Longrightarrow>
+    length \<D>s = length (const_ty_vars (\<C> f)) \<Longrightarrow>
     (\<And>\<D>. \<D> \<in> list.set \<D>s \<Longrightarrow> \<D> \<in> \<U>) \<Longrightarrow>
-    list_all2 (\<lambda>a \<tau>. a \<in> elts (denotation_ty \<xi>\<^sub>t\<^sub>y \<J>\<^sub>t\<^sub>y \<tau>)) as \<tau>s \<Longrightarrow>
-    \<J> f \<D>s as \<in> elts (denotation_ty \<xi>\<^sub>t\<^sub>y \<J>\<^sub>t\<^sub>y v)"
+    list_all2 (\<lambda>a \<tau>. a \<in> elts (denotation_ty \<xi>\<^sub>t\<^sub>y \<J>\<^sub>t\<^sub>y \<tau>)) as (const_ty_dom (\<C> f)) \<Longrightarrow>
+    \<J> f \<D>s as \<in> elts (denotation_ty \<xi>\<^sub>t\<^sub>y \<J>\<^sub>t\<^sub>y (const_ty_codom (\<C> f)))"
   assumes \<J>_True: "
     \<J> True_tconst [] [] = 1"
   assumes \<J>_False: "
@@ -151,20 +133,20 @@ locale interp_fun = type_interp \<U> \<J>\<^sub>t\<^sub>y
   assumes \<J>_Neq: "\<D> \<in> \<U> \<Longrightarrow> c \<in> elts \<D> \<Longrightarrow> d \<in> elts \<D> \<Longrightarrow>
     \<J> Neq_tconst [] [c, d] = (if c = d then 0 else 1)"
 
-type_synonym ('\<V>\<^sub>t\<^sub>y, '\<Sigma>\<^sub>t\<^sub>y, '\<V>, '\<Sigma>) lambda_designation_fun =
-  "('\<V>\<^sub>t\<^sub>y \<Rightarrow> V) \<Rightarrow> ('\<V> \<Rightarrow> V) \<Rightarrow> (('\<V>\<^sub>t\<^sub>y, '\<Sigma>\<^sub>t\<^sub>y) ty, '\<Sigma>, '\<V>) preterm \<Rightarrow> V"
+type_synonym ('\<Sigma>\<^sub>t\<^sub>y, '\<V>\<^sub>t\<^sub>y, '\<Sigma>, '\<V>) lambda_designation_fun =
+  "('\<V>\<^sub>t\<^sub>y \<Rightarrow> V) \<Rightarrow> ('\<V> \<Rightarrow> V) \<Rightarrow> (('\<Sigma>\<^sub>t\<^sub>y, '\<V>\<^sub>t\<^sub>y) ty, '\<Sigma>, '\<V>) preterm \<Rightarrow> V"
 
 locale lambda_designation = type_interp \<U> \<J>\<^sub>t\<^sub>y
   for \<U> and \<J>\<^sub>t\<^sub>y :: "('\<Sigma>\<^sub>t\<^sub>y :: type_signature) type_interp_fun" +
-  fixes \<C> :: "'\<Sigma> \<Rightarrow> ('\<V>\<^sub>t\<^sub>y, '\<Sigma>\<^sub>t\<^sub>y) const_ty"
-  fixes \<L> :: "('\<V>\<^sub>t\<^sub>y, '\<Sigma>\<^sub>t\<^sub>y, '\<V>, '\<Sigma>) lambda_designation_fun"
-  assumes "\<And>(\<xi>\<^sub>t\<^sub>y :: '\<V>\<^sub>t\<^sub>y \<Rightarrow> V) (\<xi>\<^sub>t\<^sub>e :: '\<V> \<Rightarrow> V) (\<F> :: '\<V> \<Rightarrow> ('\<V>\<^sub>t\<^sub>y, '\<Sigma>\<^sub>t\<^sub>y) ty) t \<tau>.
+  fixes \<C> :: "'\<Sigma> \<Rightarrow> ('\<Sigma>\<^sub>t\<^sub>y, '\<V>\<^sub>t\<^sub>y) const_ty"
+  fixes \<L> :: "('\<Sigma>\<^sub>t\<^sub>y, '\<V>\<^sub>t\<^sub>y, '\<Sigma>, '\<V>) lambda_designation_fun"
+  assumes "\<And>(\<xi>\<^sub>t\<^sub>y :: '\<V>\<^sub>t\<^sub>y \<Rightarrow> V) (\<xi>\<^sub>t\<^sub>e :: '\<V> \<Rightarrow> V) (\<F> :: '\<V> \<Rightarrow> ('\<Sigma>\<^sub>t\<^sub>y, '\<V>\<^sub>t\<^sub>y) ty) t \<tau>.
     type_valuation \<U> \<xi>\<^sub>t\<^sub>y \<Longrightarrow> term_valuation \<U> \<J>\<^sub>t\<^sub>y \<xi>\<^sub>t\<^sub>y \<xi>\<^sub>t\<^sub>e \<Longrightarrow>
     has_type \<C> t \<tau> \<Longrightarrow> is_Abs t \<Longrightarrow>
     \<L> \<xi>\<^sub>t\<^sub>y \<xi>\<^sub>t\<^sub>e t \<in> elts (denotation_ty \<xi>\<^sub>t\<^sub>y \<J>\<^sub>t\<^sub>y \<tau>)"
   assumes \<L>_depends_only_on_\<xi>_on_vars:
     "\<And>(\<xi>\<^sub>t\<^sub>y :: '\<V>\<^sub>t\<^sub>y \<Rightarrow> V) (\<xi>\<^sub>t\<^sub>y' :: '\<V>\<^sub>t\<^sub>y \<Rightarrow> V) (\<xi>\<^sub>t\<^sub>e :: '\<V> \<Rightarrow> V) (\<xi>\<^sub>t\<^sub>e' :: '\<V> \<Rightarrow> V) t.
-    (\<And>\<tau> x. \<tau> \<in> type_symbols t \<Longrightarrow> x \<in> type_vars \<tau> \<Longrightarrow> \<xi>\<^sub>t\<^sub>y x = \<xi>\<^sub>t\<^sub>y' x) \<Longrightarrow>
+    (\<And>\<tau> x. \<tau> \<in> type_symbols t \<Longrightarrow> x \<in> free_vars_ty \<tau> \<Longrightarrow> \<xi>\<^sub>t\<^sub>y x = \<xi>\<^sub>t\<^sub>y' x) \<Longrightarrow>
     (\<And>x. x \<in> free_vars t \<Longrightarrow> \<xi>\<^sub>t\<^sub>e x = \<xi>\<^sub>t\<^sub>e' x) \<Longrightarrow> \<L> \<xi>\<^sub>t\<^sub>y \<xi>\<^sub>t\<^sub>e t = \<L> \<xi>\<^sub>t\<^sub>y' \<xi>\<^sub>t\<^sub>e' t"
 
 locale interp =
@@ -173,15 +155,15 @@ locale interp =
   lambda_designation \<U> \<J>\<^sub>t\<^sub>y \<C> \<L>
   for \<U> and
     \<J>\<^sub>t\<^sub>y :: "('\<Sigma>\<^sub>t\<^sub>y :: type_signature) type_interp_fun" and
-    \<C> :: "'\<Sigma> :: term_signature \<Rightarrow> ('\<V>\<^sub>t\<^sub>y, '\<Sigma>\<^sub>t\<^sub>y) const_ty" and
+    \<C> :: "'\<Sigma> :: term_signature \<Rightarrow> ('\<Sigma>\<^sub>t\<^sub>y, '\<V>\<^sub>t\<^sub>y) const_ty" and
     \<J> :: "'\<Sigma> term_interp_fun" and
-    \<L> :: "('\<V>\<^sub>t\<^sub>y, '\<Sigma>\<^sub>t\<^sub>y, '\<V>, '\<Sigma>) lambda_designation_fun"
+    \<L> :: "('\<Sigma>\<^sub>t\<^sub>y, '\<V>\<^sub>t\<^sub>y, '\<Sigma>, '\<V>) lambda_designation_fun"
 
 primrec denotation_preterm ::
   "('\<V>\<^sub>t\<^sub>y \<Rightarrow> V) \<Rightarrow> ('\<V> \<Rightarrow> V) \<Rightarrow>
     ('\<Sigma>\<^sub>t\<^sub>y :: arity) type_interp_fun \<Rightarrow> '\<Sigma> term_interp_fun \<Rightarrow>
-    ('\<V>\<^sub>t\<^sub>y, '\<Sigma>\<^sub>t\<^sub>y, '\<V>, '\<Sigma>) lambda_designation_fun \<Rightarrow>
-    (('\<V>\<^sub>t\<^sub>y, '\<Sigma>\<^sub>t\<^sub>y) ty, '\<Sigma>, '\<V>) preterm \<Rightarrow> V" where
+    ('\<Sigma>\<^sub>t\<^sub>y, '\<V>\<^sub>t\<^sub>y, '\<Sigma>, '\<V>) lambda_designation_fun \<Rightarrow>
+    (('\<Sigma>\<^sub>t\<^sub>y, '\<V>\<^sub>t\<^sub>y) ty, '\<Sigma>, '\<V>) preterm \<Rightarrow> V" where
   "denotation_preterm \<xi>\<^sub>t\<^sub>y \<xi>\<^sub>t\<^sub>e \<J>\<^sub>t\<^sub>y \<J> \<L> (Free x \<tau>) = \<xi>\<^sub>t\<^sub>e x" |
   "denotation_preterm \<xi>\<^sub>t\<^sub>y \<xi>\<^sub>t\<^sub>e \<J>\<^sub>t\<^sub>y \<J> \<L> (Const f \<tau>s ts) =
     \<J> f (map (denotation_ty \<xi>\<^sub>t\<^sub>y \<J>\<^sub>t\<^sub>y) \<tau>s) (map (denotation_preterm \<xi>\<^sub>t\<^sub>y \<xi>\<^sub>t\<^sub>e \<J>\<^sub>t\<^sub>y \<J> \<L>) ts)" |
@@ -194,37 +176,25 @@ primrec denotation_preterm ::
 subsection \<open>Denotation of ground terms\<close>
 
 lemma (in type_interp) denotation_ty_of_ground:
-  assumes "type_vars \<tau> = {}"
+  assumes "free_vars_ty \<tau> = {}"
   shows "denotation_ty \<xi>\<^sub>t\<^sub>y \<J>\<^sub>t\<^sub>y \<tau> = denotation_ty \<xi>\<^sub>t\<^sub>y' \<J>\<^sub>t\<^sub>y \<tau>"
-proof (cases \<tau>)
-  case (Abs_ty \<tau>')
-
-  then have "type_vars_prety \<tau>' = {}"
-    using assms
-    by (metis Abs_ty_inverse type_vars.rep_eq)
-
-  then have "denotation_prety \<xi>\<^sub>t\<^sub>y \<J>\<^sub>t\<^sub>y \<tau>' = denotation_prety \<xi>\<^sub>t\<^sub>y' \<J>\<^sub>t\<^sub>y \<tau>'"
-  proof (induction \<tau>')
-    case (PretyVar x)
-    then have False
-      by simp
-    then show ?case ..
-  next
-    case (PretyCtr \<kappa> \<pi>s)
-    then have "denotation_prety \<xi>\<^sub>t\<^sub>y \<J>\<^sub>t\<^sub>y \<pi> = denotation_prety \<xi>\<^sub>t\<^sub>y' \<J>\<^sub>t\<^sub>y \<pi>"
-      if "\<pi> \<in> list.set \<pi>s" for \<pi>
-      using that by simp
-    then show ?case
-      by (metis (no_types, lifting) map_eq_conv denotation_prety.simps(2))
-  qed
-
-  then show ?thesis
-    using Abs_ty
-    by (simp add: Abs_ty_inverse denotation_ty_def)
+  using assms
+proof (induction \<tau>)
+  case (TyVar x)
+  then have False
+    by simp
+  then show ?case ..
+next
+  case (TyCtr \<kappa>_\<pi>s)
+  have "denotation_ty \<xi>\<^sub>t\<^sub>y \<J>\<^sub>t\<^sub>y \<pi> = denotation_ty \<xi>\<^sub>t\<^sub>y' \<J>\<^sub>t\<^sub>y \<pi>"
+    if "\<pi> \<in> set_ty_comb \<kappa>_\<pi>s" for \<pi>
+    using TyCtr that by simp
+  then show ?case
+    by (simp cong: ty_comb.map_cong)
 qed
 
 lemma (in interp) denotation_preterm_of_ground:
-  assumes "free_vars t = {}" and "(\<Union>\<tau> \<in> type_symbols t. type_vars \<tau>) = {}"
+  assumes "free_vars t = {}" and "(\<Union>\<tau> \<in> type_symbols t. free_vars_ty \<tau>) = {}"
   shows "denotation_preterm \<xi>\<^sub>t\<^sub>y \<xi>\<^sub>t\<^sub>e \<J>\<^sub>t\<^sub>y \<J> \<L> t = denotation_preterm \<xi>\<^sub>t\<^sub>y' \<xi>\<^sub>t\<^sub>e' \<J>\<^sub>t\<^sub>y \<J> \<L> t"
   using assms
 proof (induction t)
@@ -247,7 +217,7 @@ next
   case (Abs \<tau> t)
   have "\<L> \<xi>\<^sub>t\<^sub>y \<xi>\<^sub>t\<^sub>e (Abs \<tau> t) = \<L> \<xi>\<^sub>t\<^sub>y' \<xi>\<^sub>t\<^sub>e' (Abs \<tau> t)"
   proof (rule \<L>_depends_only_on_\<xi>_on_vars)
-    show "\<And>\<tau>' x. \<tau>' \<in> type_symbols (Abs \<tau> t) \<Longrightarrow> x \<in> type_vars \<tau>' \<Longrightarrow> \<xi>\<^sub>t\<^sub>y x = \<xi>\<^sub>t\<^sub>y' x"
+    show "\<And>\<tau>' x. \<tau>' \<in> type_symbols (Abs \<tau> t) \<Longrightarrow> x \<in> free_vars_ty \<tau>' \<Longrightarrow> \<xi>\<^sub>t\<^sub>y x = \<xi>\<^sub>t\<^sub>y' x"
       using Abs.prems(2) by blast
   next
     show "\<And>x. x \<in> free_vars (Abs \<tau> t) \<Longrightarrow> \<xi>\<^sub>t\<^sub>e x = \<xi>\<^sub>t\<^sub>e' x"
@@ -265,14 +235,16 @@ locale proper_interp = interp +
   assumes "app (\<L> \<xi>\<^sub>t\<^sub>y \<xi> (Abs \<tau> t)) a = \<L> \<xi>\<^sub>t\<^sub>y (\<xi>(x := a)) (open_bound 0 \<tau> (Free x \<tau>) t)"
 
 declare [[typedef_overloaded]]
-record ('\<V>\<^sub>t\<^sub>y, '\<Sigma>\<^sub>t\<^sub>y :: arity, '\<V>, '\<Sigma>) interp =
+record ('\<Sigma>\<^sub>t\<^sub>y :: arity, '\<V>\<^sub>t\<^sub>y, '\<Sigma>, '\<V>) interp =
   \<U> :: "V set"
-  \<C> :: "'\<Sigma> \<Rightarrow> ('\<V>\<^sub>t\<^sub>y, '\<Sigma>\<^sub>t\<^sub>y) const_ty"
+  \<C> :: "'\<Sigma> \<Rightarrow> ('\<Sigma>\<^sub>t\<^sub>y, '\<V>\<^sub>t\<^sub>y) const_ty"
   \<J>\<^sub>t\<^sub>y :: "'\<Sigma>\<^sub>t\<^sub>y \<Rightarrow> V list \<Rightarrow> V"
   \<J> :: "'\<Sigma> \<Rightarrow> V list \<Rightarrow> V list \<Rightarrow> V"
-  \<L> :: "('\<V>\<^sub>t\<^sub>y \<Rightarrow> V) \<Rightarrow> ('\<V> \<Rightarrow> V) \<Rightarrow> (('\<V>\<^sub>t\<^sub>y, '\<Sigma>\<^sub>t\<^sub>y) ty, '\<Sigma>, '\<V>) preterm \<Rightarrow> V"
+  \<L> :: "('\<V>\<^sub>t\<^sub>y \<Rightarrow> V) \<Rightarrow> ('\<V> \<Rightarrow> V) \<Rightarrow> (('\<Sigma>\<^sub>t\<^sub>y, '\<V>\<^sub>t\<^sub>y) ty, '\<Sigma>, '\<V>) preterm \<Rightarrow> V"
 
-type_synonym ('\<V>\<^sub>t\<^sub>y, '\<Sigma>\<^sub>t\<^sub>y, '\<V>, '\<Sigma>) atom = "(('\<V>\<^sub>t\<^sub>y, '\<Sigma>\<^sub>t\<^sub>y) ty, '\<Sigma>, '\<V>) preterm uprod"
+type_synonym ('\<Sigma>\<^sub>t\<^sub>y, '\<V>\<^sub>t\<^sub>y, '\<Sigma>, '\<V>) atom =
+  "(('\<Sigma>\<^sub>t\<^sub>y, '\<V>\<^sub>t\<^sub>y) ty, '\<Sigma>, '\<V>) preterm uprod"
+
 datatype 'a literal =
   is_pos: Pos (atom: 'a) |
   is_neg: Neg (atom: 'a)
@@ -289,8 +261,8 @@ instance ..
 end
 
 fun true_lit ::
-  "('\<V>\<^sub>t\<^sub>y, '\<Sigma>\<^sub>t\<^sub>y :: arity, '\<V>, '\<Sigma>) interp \<times> ('\<V>\<^sub>t\<^sub>y \<Rightarrow> V) \<times> ('\<V> \<Rightarrow> V) \<Rightarrow>
-    ('\<V>\<^sub>t\<^sub>y, '\<Sigma>\<^sub>t\<^sub>y, '\<V>, '\<Sigma>) atom literal \<Rightarrow> bool"
+  "('\<Sigma>\<^sub>t\<^sub>y :: arity, '\<V>\<^sub>t\<^sub>y, '\<Sigma>, '\<V>) interp \<times> ('\<V>\<^sub>t\<^sub>y \<Rightarrow> V) \<times> ('\<V> \<Rightarrow> V) \<Rightarrow>
+    ('\<Sigma>\<^sub>t\<^sub>y, '\<V>\<^sub>t\<^sub>y, '\<Sigma>, '\<V>) atom literal \<Rightarrow> bool"
   (infix \<open>\<Turnstile>\<^sub>l\<close> 50) where
   "(\<I>, \<xi>\<^sub>t\<^sub>y, \<xi>\<^sub>t\<^sub>e) \<Turnstile>\<^sub>l (Pos A) \<longleftrightarrow> (case_uprod (Abs_commute (=))
     (map_uprod (denotation_preterm \<xi>\<^sub>t\<^sub>y \<xi>\<^sub>t\<^sub>e (interp.\<J>\<^sub>t\<^sub>y \<I>) (interp.\<J> \<I>) (interp.\<L> \<I>)) A))" |
@@ -307,14 +279,14 @@ lemma not_true_lit_Neg_ident: "\<not> (\<I>\<xi> \<Turnstile>\<^sub>l (Neg (Upai
   by (cases \<I>\<xi>) simp
 
 definition true_cls ::
-  "('\<V>\<^sub>t\<^sub>y, '\<Sigma>\<^sub>t\<^sub>y :: arity, '\<V>, '\<Sigma>) interp \<times> ('\<V>\<^sub>t\<^sub>y \<Rightarrow> V) \<times> ('\<V> \<Rightarrow> V) \<Rightarrow>
-    ('\<V>\<^sub>t\<^sub>y, '\<Sigma>\<^sub>t\<^sub>y, '\<V>, '\<Sigma>) atom literal multiset \<Rightarrow> bool"
+  "('\<Sigma>\<^sub>t\<^sub>y :: arity, '\<V>\<^sub>t\<^sub>y, '\<Sigma>, '\<V>) interp \<times> ('\<V>\<^sub>t\<^sub>y \<Rightarrow> V) \<times> ('\<V> \<Rightarrow> V) \<Rightarrow>
+    ('\<Sigma>\<^sub>t\<^sub>y, '\<V>\<^sub>t\<^sub>y, '\<Sigma>, '\<V>) atom literal multiset \<Rightarrow> bool"
   (infix \<open>\<Turnstile>\<^sub>c\<close> 50) where
   "\<I>\<xi> \<Turnstile>\<^sub>c C \<longleftrightarrow> (\<exists>L \<in># C. \<I>\<xi> \<Turnstile>\<^sub>l L)"
 
 definition true_clss ::
-  "('\<V>\<^sub>t\<^sub>y, '\<Sigma>\<^sub>t\<^sub>y :: type_signature, '\<V>, '\<Sigma> :: term_signature) interp \<Rightarrow>
-    ('\<V>\<^sub>t\<^sub>y, '\<Sigma>\<^sub>t\<^sub>y, '\<V>, '\<Sigma>) atom literal multiset set \<Rightarrow> bool"
+  "('\<Sigma>\<^sub>t\<^sub>y :: type_signature, '\<V>\<^sub>t\<^sub>y, '\<Sigma> :: term_signature, '\<V>) interp \<Rightarrow>
+    ('\<Sigma>\<^sub>t\<^sub>y, '\<V>\<^sub>t\<^sub>y, '\<Sigma>, '\<V>) atom literal multiset set \<Rightarrow> bool"
   (infix \<open>\<Turnstile>\<^sub>c\<^sub>s\<close> 50) where
   "\<I> \<Turnstile>\<^sub>c\<^sub>s N \<longleftrightarrow>
     proper_interp (interp.\<U> \<I>) (interp.\<J>\<^sub>t\<^sub>y \<I>) (interp.\<C> \<I>) (interp.\<J> \<I>) (interp.\<L> \<I>) \<and>
